src/cddl/pulse/CDDL.Pulse.Serialize.Gen.MapGroup.Ext.fst
@@ -1,0 +1,52 @@
+module CDDL.Pulse.Serialize.Gen.MapGroup.Ext
+#lang-pulse
+
+module GR = Pulse.Lib.GhostReference
+module Map = CDDL.Spec.Map
+
+(* impl_serialize_map_group_ext *)
+
+inline_for_extraction noextract [@@noextract_to "krml"]
+fn impl_serialize_map_group_ext
+  (#p: Ghost.erased bare_cbor_map_parser)
+  (#minl: Ghost.erased (cbor -> nat))
+  (#maxl: Ghost.erased (cbor -> option nat))
+    (#[@@@erasable]t: Ghost.erased (det_map_group))
+    (# [@@@erasable] fp: Ghost.erased map_constraint)
+    (#[@@@erasable]tgt: Type0)
+    (#[@@@erasable] inj: Ghost.erased bool)
+    (#[@@@erasable]ps: Ghost.erased (mg_spec t fp tgt inj))
+    (#impl_tgt: Type0)
+    (#[@@@erasable]r: rel impl_tgt tgt)
+    (i: impl_serialize_map_group p minl maxl ps r)
+    (#[@@@erasable]t': Ghost.erased (det_map_group))
+    (# [@@@erasable] fp': Ghost.erased map_constraint)
+    (#[@@@erasable] inj': Ghost.erased bool)
+    ([@@@erasable]ps': Ghost.erased (mg_spec t' fp' tgt inj'))
+    ([@@@erasable]sq: squash (
+      t' == t /\
+      (forall (x: tgt) . (Ghost.reveal ps').mg_serializable x <==> (Ghost.reveal ps).mg_serializable x) /\
+      (forall (x: tgt) . (Ghost.reveal ps').mg_serializable x ==> (
+        (Ghost.reveal ps).mg_serializable x /\
+        (Ghost.reveal ps').mg_serializer x `cbor_map_equal` (Ghost.reveal ps).mg_serializer x
+      )) /\
+      (forall (x: tgt) . (Ghost.reveal ps').mg_size x == (Ghost.reveal ps).mg_size x)
+    ))
+: impl_serialize_map_group p minl maxl #(Ghost.reveal t') #(Ghost.reveal fp') #tgt #inj' (Ghost.reveal ps') #impl_tgt r
+=
+    (c: _)
+    (#v: _)
+    (out: _)
+    (out_count: _)
+    (out_size: _)
+    (l: _)
+{
+  i c out out_count out_size l
+}
+
+(* impl_serialize_map_group_ext' *)
+
+inline_for_extraction noextract [@@noextract_to "krml"]
+let impl_serialize_map_group_ext'
+  #p #minl #maxl #t #fp #tgt #inj #ps #impl_tgt #r i fp' sq
+= impl_serialize_map_group_ext i _ ()
